new/proof/github_com/goose_lang/goose/model/channel/logatom/chan_au_send.v
@@ -264,8 +264,8 @@ Proof.
     iNamed "phys". iNamed "offer". wp_auto. unfold chan_cap_valid in Hcapvalid.
     wp_if_destruct.
     {
-      iDestruct (slice_array with "tmp") as "Hsl"; first done.
-      rewrite go.array_index_ref_0 /=.
+      wp_apply wp_slice_literal as "%sl Hsl".
+      { iIntros. by wp_auto. }
       iDestruct (own_slice_len with "slice") as "[%Hl %Hcap2]".
       iDestruct (slice.own_slice_len with "slice") as "[%Hlen_slice %Hslgtz]".
       iDestruct (own_slice_wf with "slice") as "%Hwf".
@@ -511,9 +511,8 @@ Proof.
       { simpl in *. len. }
       { simpl in *. len. }
       iMod ("Hcont" with "Hchanrepfrag") as "Hstep". iModIntro.
-      iDestruct (slice_array with "tmp") as "Hsl".
-      { done. }
-      rewrite go.array_index_ref_0.
+      wp_apply wp_slice_literal as "%sl Hsl".
+      { iIntros. by wp_auto. }
       wp_apply (wp_slice_append with "[$slice_inv $Hsl $slice_cap_inv]").
       iIntros (fr) "(slice_inv & slice_cap_inv & Hsl)". wp_auto.
       iCombineNamed "*_inv" as "Hi".
@@ -626,8 +625,8 @@ Proof.
       destruct decide.
       2:{ exfalso. word. }
       iMod ("Hcont" with "Hchanrepfrag") as "Hstep". iModIntro.
-      iDestruct (slice_array with "tmp") as "Hsl"; first done.
-      rewrite go.array_index_ref_0.
+      wp_apply wp_slice_literal as "%sl Hsl".
+      { iIntros. by wp_auto. }
       wp_apply (wp_slice_append with "[$slice_inv $Hsl $slice_cap_inv]").
       iIntros (fr) "(slice_inv & slice_cap_inv & Hsl)". wp_auto.
       iCombineNamed "*_inv" as "Hi".
